Tau_Sink_Contrasim.thy
@@ -8,23 +8,14 @@ begin
 context lts_tau
 begin
 
-definition trace_simulation ::
-  \<open>('s \<Rightarrow> 's \<Rightarrow> bool) \<Rightarrow> bool\<close>
-where
-  \<open>trace_simulation R  \<equiv> \<forall> p q p' A . (\<forall> a \<in> set(A). a \<noteq> \<tau>) 
-  \<and> R p q \<and> p \<Rightarrow>$ A p' \<longrightarrow> (\<exists> q'. q \<Rightarrow>$ A q')\<close>
-
-lemma contrasim_implies_trace_sim:
-  assumes \<open>contrasim R\<close>
-  shows \<open>trace_simulation R\<close>
-by (metis assms contrasim_simpler_def trace_simulation_def) 
+section \<open>Similarity ignores \<open>\<tau>\<close>-sinks\<close>
 
 definition tau_sink ::
   \<open>'s \<Rightarrow> bool\<close>
 where
   \<open>tau_sink p  \<equiv> \<forall>a. \<nexists>p'. p \<longmapsto>a p'\<close>
 
-lemma tau_sink_has_no_weak_transitions: 
+lemma sink_has_no_weak_transitions: 
   assumes 
     \<open>tau_sink sink\<close>
   shows \<open>\<nexists>s'. s' \<noteq> sink \<and> sink \<Rightarrow>^a s'\<close>
@@ -33,7 +24,7 @@ proof -
   show ?thesis by (metis assms lts_tau.tau_sink_def stable_tauclosure_only_loop) 
 qed
 
-lemma tau_sink_has_no_word_transitions: 
+lemma sink_has_no_word_transitions: 
   assumes 
     \<open>tau_sink sink\<close>
     \<open>A \<noteq> []\<close>
@@ -42,11 +33,287 @@ lemma tau_sink_has_no_word_transitions:
 proof - 
   obtain a where \<open>\<exists>B. A = a#B\<close> using assms(2) list.exhaust_sel by auto
   hence \<open>\<nexists>s' . sink \<Rightarrow>^a s'\<close>
-    by (metis assms(1, 3) list.set_intros(1) lts_tau.tau_def tau_sink_def tau_sink_has_no_weak_transitions)
+    by (metis assms(1, 3) list.set_intros(1) lts_tau.tau_def tau_sink_def sink_has_no_weak_transitions)
   thus ?thesis using \<open>\<exists>B. A = a#B\<close> by fastforce
 qed
+  
+lemma simulation_tau_sink_1:
+  fixes
+    step sink R
+  defines
+    \<open>step2 \<equiv> \<lambda> p1 a p2 . (p1 \<noteq> sink \<and> a = \<tau> \<and> p2 = sink) \<or> step p1 a p2\<close>
+  assumes
+    \<open>\<And> a p . \<not> step sink a p\<close>
+    \<open>lts_tau.weak_simulation step \<tau> R\<close>
+  shows
+    \<open>lts_tau.weak_simulation step2 \<tau> (\<lambda> p q. p = sink \<or> R p q)\<close>
+proof -
+  let ?tau = \<open>(lts_tau.tau \<tau>)\<close>
+  let ?tauEx = \<open>\<tau>\<close>
+  show ?thesis unfolding lts_tau.weak_simulation_def
+  proof safe
+    fix p q p' a
+    assume \<open>step2 sink a p'\<close>
+    hence \<open>p' = sink\<close> \<open>a = \<tau>\<close>
+      using assms(2) unfolding step2_def by auto
+    thus \<open>\<exists>q'. (p' = sink \<or> R p' q') \<and>
+      (?tau a \<longrightarrow> lts.steps step2 q ?tau q') \<and> 
+      (\<not> ?tau a \<longrightarrow> (\<exists>pq1 pq2. lts.steps step2 q ?tau pq1 \<and> step2 pq1 a pq2 
+        \<and> lts.steps step2 pq2 ?tau q'))\<close>
+      using lts_tau.step_tau_refl[of \<tau> step2 q] by auto
+  next
+    fix p q p' a
+    assume \<open>step2 p a p'\<close> \<open>R p q\<close>
+    have step_impl_step2: \<open>\<And> p1 a p2 . step p1 a p2 \<Longrightarrow> step2 p1 a p2\<close>
+      unfolding step2_def by blast
+    have \<open>(p \<noteq> sink \<and> a = ?tauEx \<and> p' = sink) \<or> step p a p'\<close>
+      using `step2 p a p'` unfolding step2_def .
+    thus \<open>\<exists>q'. (p' = sink \<or> R p' q') \<and>
+      (?tau a \<longrightarrow> lts.steps step2 q ?tau q') \<and>
+      (\<not> ?tau a \<longrightarrow> (\<exists>pq1 pq2. lts.steps step2 q ?tau pq1 \<and> step2 pq1 a pq2
+        \<and> lts.steps step2 pq2 ?tau q'))\<close>
+    proof safe
+      show \<open>\<exists>q'. (sink = sink \<or> R sink q') \<and>
+           (?tau ?tauEx \<longrightarrow> lts.steps step2 q ?tau q') \<and>
+           (\<not> ?tau ?tauEx \<longrightarrow> (\<exists>pq1 pq2. lts.steps step2 q ?tau pq1
+            \<and> step2 pq1 ?tauEx pq2 \<and> lts.steps step2 pq2 ?tau q'))\<close>
+        using lts.steps.refl[of step2 q ?tau] assms(1) by (meson lts_tau.tau_tau)
+    next
+      assume \<open>step p a p'\<close>
+      then obtain q' where q'_def:
+        \<open>R p' q' \<and>
+        (?tau a \<longrightarrow> lts.steps step q ?tau q') \<and>
+        (\<not> ?tau a \<longrightarrow> (\<exists>pq1 pq2. lts.steps step q ?tau pq1 \<and> step pq1 a pq2
+          \<and> lts.steps step pq2 ?tau q'))\<close>
+        using assms(3) `R p q` unfolding lts_tau.weak_simulation_def by blast
+      hence \<open>(p' = sink \<or> R p' q') \<and>
+        (?tau a \<longrightarrow> lts.steps step2 q ?tau q') \<and>
+        (\<not> ?tau a \<longrightarrow> (\<exists>pq1 pq2. lts.steps step2 q ?tau pq1 \<and> step2 pq1 a pq2
+          \<and> lts.steps step2 pq2 ?tau q'))\<close>
+        using lts_impl_steps[of step _ _ _ step2] step_impl_step2 by blast
+      thus \<open>\<exists>q'. (p' = sink \<or> R p' q') \<and>
+        (?tau a \<longrightarrow> lts.steps step2 q ?tau q') \<and>
+        (\<not> ?tau a \<longrightarrow> (\<exists>pq1 pq2. lts.steps step2 q ?tau pq1 \<and> step2 pq1 a pq2
+          \<and> lts.steps step2 pq2 ?tau q'))\<close>
+        by blast
+    qed
+  qed
+qed
+  
+lemma simulation_tau_sink_2:
+  fixes
+    step sink R 
+  defines
+    \<open>step2 \<equiv> \<lambda> p1 a p2 . (p1 \<noteq> sink \<and> a = \<tau> \<and> p2 = sink) \<or> step p1 a p2\<close>
+  assumes
+    \<open>\<And> a p . \<not> step sink a p \<and> \<not> step p a sink\<close>
+    \<open>lts_tau.weak_simulation step2 \<tau> (\<lambda> p q. p = sink \<or> R p q)\<close>
+    \<open>\<And> p' q' q . (p' = sink \<or> R p' q') 
+      \<and> lts.steps step2 q (lts_tau.tau \<tau>) q'  \<longrightarrow> (p' = sink \<or> R p' q)\<close>
+  shows
+    \<open>lts_tau.weak_simulation step \<tau> (\<lambda> p q. p = sink \<or> R p q)\<close>
+proof -
+  let ?tau = \<open>(lts_tau.tau \<tau>)\<close>
+  let ?tauEx = \<open>\<tau>\<close>
+  let ?steps = \<open>lts.steps\<close>
+  show ?thesis
+    unfolding lts_tau.weak_simulation_def
+  proof safe
+    fix p q p' a
+    assume
+      \<open>step sink a p'\<close>
+    hence False using assms(2) by blast
+    thus \<open>\<exists>q'. (p' = sink \<or> R p' q') \<and>
+      (?tau a \<longrightarrow> ?steps step q ?tau q') \<and>
+      (\<not> ?tau a \<longrightarrow> (\<exists>pq1 pq2. ?steps step q ?tau pq1 \<and> step pq1 a pq2
+        \<and> ?steps step pq2 ?tau q'))\<close> ..
+  next
+    fix p q p' a
+    assume \<open>R p q\<close> \<open>step p a p'\<close>
+    hence not_sink: \<open>p \<noteq> sink\<close> \<open>p' \<noteq> sink\<close>
+      using assms(2)[of a p] assms(2)[of a p'] by auto
+    have \<open>step2 p a p'\<close> using `step p a p'` unfolding step2_def by blast
+    then obtain q' where q'_def:
+      \<open>p' = sink \<or> R p' q'\<close>
+      \<open>?tau a \<longrightarrow> ?steps step2 q ?tau q'\<close>  
+      \<open>\<not> ?tau a \<longrightarrow> (\<exists>pq1 pq2. ?steps step2 q ?tau pq1 \<and> step2 pq1 a pq2 
+        \<and> ?steps step2 pq2 ?tau q')\<close>
+      using assms(3) `R p q` unfolding lts_tau.weak_simulation_def by blast
+    hence outer_goal_a: \<open>R p' q'\<close> using not_sink by blast
+    show \<open>\<exists>q'. (p' = sink \<or> R p' q') \<and>
+      (?tau a \<longrightarrow> ?steps step q ?tau q') \<and>
+      (\<not> ?tau a \<longrightarrow> (\<exists>pq1 pq2. ?steps step q ?tau pq1 \<and> step pq1 a pq2
+        \<and> ?steps step pq2 ?tau q'))\<close>
+    proof (cases \<open>q' = sink\<close>)
+      assume \<open>q' = sink\<close>
+      then obtain q'' where q''_def:
+        \<open>?tau a \<longrightarrow> (?steps step q ?tau q'' \<and> ?steps step2 q'' ?tau q')\<close>
+        \<open>\<not> ?tau a \<longrightarrow> (\<exists>pq1. ?steps step2 q ?tau pq1 \<and> step pq1 a q''
+          \<and> ?steps step2 q'' ?tau q')\<close>
+        using q'_def(2,3) assms(1) step2_def lts_tau.step_tau_refl[of \<tau>]
+          lts_tau.tau_tau[of \<tau>] by metis
+      hence \<open>q'' = sink \<longrightarrow> q = sink\<close>
+        using assms(2) unfolding step2_def by (metis lts.steps.cases)
+      have \<open>?steps step2 q'' ?tau q'\<close> using q''_def by auto
+      hence \<open>p' = sink \<or> R p' q''\<close> using  q'_def(1) assms(4)[of p' q' q''] by blast
+      moreover have \<open>\<not> ?tau a \<longrightarrow> (\<exists>pq1 pq2. ?steps step q ?tau pq1 \<and> step pq1 a pq2
+        \<and> ?steps step pq2 ?tau q'')\<close>
+      proof
+        assume \<open>\<not> ?tau a\<close>
+        hence \<open>q \<noteq> sink\<close> using q'_def by (metis assms(2) lts.steps_left step2_def)
+        hence \<open>q'' \<noteq> sink\<close> using `q'' = sink \<longrightarrow> q = sink` by simp
+        obtain pq1 where pq1_def:
+            \<open>?steps step2 q ?tau pq1\<close> \<open>step pq1 a q''\<close> \<open>?steps step2 q'' ?tau q'\<close>
+          using q''_def(2) `\<not> ?tau a` by blast
+        hence \<open>pq1 \<noteq> sink\<close> using `q'' \<noteq> sink` assms(2) by blast
+        hence \<open>?steps step q ?tau pq1\<close> using `q \<noteq> sink` `?steps step2 q ?tau pq1`
+        proof (induct rule: lts.steps.induct[OF `?steps step2 q ?tau pq1`])
+          case (1 p af)
+          then show ?case using lts.steps.refl[of step p af] by blast
+        next
+          case (2 p af q1 a q)
+          hence \<open>q1 \<noteq> sink\<close> \<open>step q1 a q\<close> using assms(2) unfolding step2_def by auto
+          moreover hence \<open>?steps step p af q1\<close> using 2 by blast 
+          ultimately show ?case using 2(4) by (meson lts.step)
+        qed
+        thus
+          \<open>\<exists>pq1 pq2. ?steps step q ?tau pq1 \<and> step pq1 a pq2 \<and> ?steps step pq2 ?tau q''\<close>
+          using pq1_def(2) lts.steps.refl[of step q'' ?tau] by blast
+      qed
+      ultimately show \<open>\<exists>q''. (p' = sink \<or> R p' q'') \<and>
+           (?tau a \<longrightarrow> ?steps step q ?tau q'') \<and>
+           (\<not> ?tau a \<longrightarrow> (\<exists>pq1 pq2. ?steps step q ?tau pq1 \<and> step pq1 a pq2
+            \<and> ?steps step pq2 ?tau q''))\<close>
+        using q''_def(1) q'_def(1) by auto
+    next
+      assume not_sink_q': \<open>q' \<noteq> sink\<close>
+      have outer_goal_b: \<open>?tau a \<longrightarrow> ?steps step q ?tau q'\<close>
+        using q'_def(2) not_sink_q' unfolding step2_def
+      proof (safe)
+        assume i:
+          \<open>q' \<noteq> sink\<close> \<open>?tau a\<close>
+          \<open>?steps (\<lambda>p1 a p2.  p1 \<noteq> sink \<and> a = ?tauEx \<and> p2 = sink \<or> step p1 a p2) q ?tau q'\<close>
+        thus \<open>?steps step q ?tau q'\<close>
+        proof (induct rule: lts.steps.induct[OF i(3)])
+          case (1 p af)
+          then show ?case using lts.steps.refl[of _ p af] by auto
+        next
+          case (2 p af q1 a q)
+          hence \<open>step q1 a q\<close> by blast
+          moreover have \<open>?steps step p af q1\<close> using 2 assms(2) by blast
+          ultimately show ?case using `af a` lts.step[of step p af q1 a q] by blast
+        qed
+      qed
+      have outer_goal_c:
+          \<open>\<not> ?tau a \<longrightarrow> (\<exists>pq1 pq2. ?steps step q ?tau pq1 \<and> step pq1 a pq2
+          \<and> ?steps step pq2 ?tau q')\<close>
+        using q'_def(3)
+      proof safe
+        fix pq1 pq2
+        assume subassms:
+          \<open>\<not> ?tau a\<close>
+          \<open>?steps step2 q ?tau pq1\<close>
+          \<open>step2 pq1 a pq2\<close>
+          \<open>?steps step2 pq2 ?tau q'\<close>
+        have \<open>pq2 \<noteq> sink\<close> 
+          using subassms(4) assms(2) not_sink_q' lts.steps_loop
+          unfolding step2_def by (metis (mono_tags, lifting))
+        have  goal_c: \<open>?steps step pq2 ?tau q'\<close>
+          using subassms(4) not_sink_q' unfolding step2_def
+        proof (induct rule:lts.steps.induct[OF subassms(4)])
+          case (1 p af) show ?case using lts.steps.refl by assumption
+        next
+          case (2 p af q1 a q)
+          hence \<open>step q1 a q\<close> unfolding step2_def by simp
+          moreover hence \<open>q1 \<noteq> sink\<close> using assms(2) by blast
+          ultimately have \<open>?steps step p af q1\<close> using 2 unfolding step2_def by auto
+          thus ?case using `step q1 a q` 2(4) lts.step[of step p af q1 a q] by blast
+        qed
+        have goal_b: \<open>step pq1 a pq2\<close>
+          using `pq2 \<noteq> sink` subassms(3) unfolding step2_def by blast
+        hence \<open>pq1 \<noteq> sink\<close> using assms(2) by blast
+        hence goal_a: \<open>?steps step q ?tau pq1\<close>
+          using subassms(4) unfolding step2_def
+        proof (induct rule:lts.steps.induct[OF subassms(2)])
+          case (1 p af) show ?case using lts.steps.refl by assumption
+        next
+          case (2 p af q1 a q)
+          hence \<open>step q1 a q\<close> unfolding step2_def by simp
+          moreover hence \<open>q1 \<noteq> sink\<close> using assms(2) by blast
+          ultimately have \<open>?steps step p af q1\<close> using 2 unfolding step2_def by auto
+          thus ?case using `step q1 a q` 2(4) lts.step[of step p af q1 a q] by blast
+        qed
+        thus
+          \<open>\<exists>pq1 pq2. ?steps step q ?tau pq1 \<and> step pq1 a pq2 \<and> ?steps step pq2 ?tau q'\<close>
+          using goal_b goal_c by auto
+      qed
+      thus \<open>\<exists>q'. (p' = sink \<or> R p' q') \<and> (?tau a \<longrightarrow> ?steps step q ?tau q') \<and>
+        (\<not> ?tau a \<longrightarrow> (\<exists>pq1 pq2. ?steps step q ?tau pq1 \<and> step pq1 a pq2
+          \<and> ?steps step pq2 ?tau q'))\<close>
+        using outer_goal_a outer_goal_b by auto
+    qed
+  qed
+qed
 
-lemma tau_sink_contrasimulates_all_states:
+lemma simulation_sink_invariant:
+  fixes
+    step sink R
+  defines
+    \<open>step2 \<equiv> \<lambda> p1 a p2 . (p1 \<noteq> sink \<and> a =  \<tau> \<and> p2 = sink) \<or> step p1 a p2\<close>
+  assumes
+    \<open>\<And> a p . \<not> step sink a p \<and> \<not> step p a sink\<close>
+  shows \<open>lts_tau.weakly_simulated_by step2 \<tau> p q = lts_tau.weakly_simulated_by step \<tau> p q\<close>
+proof (rule)
+  have sink_sim_min: \<open>lts_tau.weak_simulation step2 \<tau> (\<lambda> p q. p = sink)\<close>
+    unfolding lts_tau.weak_simulation_def step2_def using assms(2)
+    by (meson lts.steps.simps)
+  define R where \<open>R \<equiv> lts_tau.weakly_simulated_by step2 \<tau>\<close>
+  have weak_sim_R: \<open>lts_tau.weak_simulation step2 \<tau> R\<close>
+    using lts_tau.weaksim_greatest[of step2 \<tau>] unfolding R_def by blast
+  have R_contains_inv_tau_closure:
+    \<open>R = (\<lambda>p1 q1. R p1 q1 \<or> lts.steps step2 q1 (lts_tau.tau \<tau>) p1)\<close> unfolding R_def
+  proof (rule, rule, rule, simp)
+    fix p q
+    assume
+      \<open>(\<exists>R. lts_tau.weak_simulation step2 \<tau>  R \<and> R p q) \<or>
+       (lts.steps step2 q (lts_tau.tau \<tau>) p)\<close>
+    thus \<open>\<exists>R. lts_tau.weak_simulation step2 \<tau> R \<and> R p q\<close>
+      using weak_sim_R
+            lts_tau.weak_sim_tau_step[of step2 \<open>\<tau>\<close>]
+            lts_tau.weak_sim_union_cl[of step2 \<open>\<tau>\<close>] by blast
+  qed
+  assume Rpq: \<open>R p q\<close>
+  have \<open>\<And> p' q' q . R p' q' \<and> lts.steps step2 q (lts_tau.tau \<tau>) q'  \<longrightarrow> R p' q\<close>
+    using R_contains_inv_tau_closure lts_tau.weak_sim_trans[of step2 \<open>\<tau>\<close> _ _ _] R_def assms(2)
+    by meson
+  hence closed_R:
+      \<open>\<And> p' q' q . (p' = sink \<or> R p' q') \<and> lts.steps step2 q (lts_tau.tau \<tau>) q'
+         \<longrightarrow> (p' = sink \<or> R p' q)\<close>
+    using weak_sim_R sink_sim_min lts_tau.weak_sim_union_cl by blast
+  have \<open>lts_tau.weak_simulation step2 \<tau> (\<lambda>p q. p = sink \<or> R p q)\<close>
+    using weak_sim_R sink_sim_min lts_tau.weak_sim_union_cl[of step2 \<tau>] by blast
+  hence \<open>lts_tau.weak_simulation step \<tau> (\<lambda>p q. p = sink \<or> R p q)\<close>
+    using  simulation_tau_sink_2[of step sink \<tau> R] assms(2) closed_R
+    unfolding step2_def by blast
+  thus \<open>\<exists>R. lts_tau.weak_simulation step \<tau> R \<and> R p q\<close>
+    using Rpq weak_sim_R by blast
+next
+  show \<open>\<exists>R. lts_tau.weak_simulation step \<tau> R \<and> R p q \<Longrightarrow>
+        \<exists>R. lts_tau.weak_simulation step2 \<tau> R \<and> R p q\<close>
+  proof clarify
+    fix R
+    assume
+      \<open>lts_tau.weak_simulation step \<tau> R\<close>
+      \<open>R p q\<close>
+    hence \<open>lts_tau.weak_simulation
+      (\<lambda>p1 a p2. p1 \<noteq> sink \<and> a = \<tau> \<and> p2 = sink \<or> step p1 a p2) \<tau> (\<lambda>p q. p = sink \<or> R p q)\<close>
+      using simulation_tau_sink_1[of step sink \<tau> R] assms(2) unfolding step2_def by auto
+    thus \<open>\<exists>R. lts_tau.weak_simulation step2 \<tau> R \<and> R p q\<close>
+      using `R p q` unfolding step2_def by blast
+  qed
+qed
+
+lemma sink_contrasimulates_all_states:
 fixes A :: " 'a list"
   assumes 
     \<open>tau_sink sink\<close>
@@ -62,11 +329,11 @@ proof (cases A)
 next
   case Cons
   hence \<open>\<nexists>s'. (\<forall> a \<in> set(A). a \<noteq> \<tau>) \<and> sink \<Rightarrow>$A s'\<close>
-    using assms(1) tau_sink_has_no_word_transitions by fastforce
+    using assms(1) sink_has_no_word_transitions by fastforce
   show ?thesis using assms(2) contrasim_tau_step by auto 
 qed
 
-lemma tau_sink_coupled_simulates_all_states:
+lemma sink_coupled_simulates_all_states:
   assumes 
     \<open>tau_sink sink\<close>
     \<open>\<And> p . (p \<longmapsto>* tau sink)\<close>
@@ -74,19 +341,19 @@ lemma tau_sink_coupled_simulates_all_states:
     \<open>sink \<sqsubseteq>cs p\<close> 
   by (simp add: assms(1, 2) coupledsim_refl tau_sink_def coupledsim_step)  
 
-lemma tau_sink_trace_sim_contrasim:
+lemma trace_incl_with_sink_is_contrasim:
   assumes
     \<open>\<And> p . (p \<longmapsto>* tau sink)\<close>
     \<open>\<And> p . R sink p\<close>
-    \<open>trace_simulation R\<close>
+    \<open>trace_inclusion R\<close>
   shows
-    \<open>contrasim R\<close>
- unfolding contrasim_def
+    \<open>contrasimulation R\<close>
+ unfolding contrasimulation_def
 proof clarify
   fix p q p' A
   assume \<open>R p q\<close> \<open>p \<Rightarrow>$A  p'\<close> \<open>\<forall> a \<in> set(A). a \<noteq> \<tau>\<close>
   hence \<open>\<exists>q'. q \<Rightarrow>$A  q'\<close>
-    using assms(3) unfolding trace_simulation_def by blast
+    using assms(3) unfolding trace_inclusion_def by blast
   hence \<open>q \<Rightarrow>$A  sink\<close>
     using assms(1) tau_tau word_tau_concat by blast
   thus \<open>\<exists>q'. q \<Rightarrow>$ A  q' \<and> R q' p'\<close>
